Use locales and obtain executable SML code

BTree_Imp.thy
@@ -44,6 +44,807 @@ fun btree_assn :: "nat \<Rightarrow> 'a::heap btree \<Rightarrow> 'a btnode ref 
   "btree_assn _ _ _ = false"
 
 
+definition "split_relation xs \<equiv> \<lambda>(as,bs) i. i \<le> length xs \<and> as = take i xs \<and> bs = drop i xs"
+
+lemma split_relation_alt: 
+  "split_relation as (ls,rs) i = (as = ls@rs \<and> i = length ls)"
+  by (auto simp add: split_relation_def)
+
+lemma split_relation_length: "split_relation xs (ls,rs) (length xs) = (ls = xs \<and> rs = [])"
+  by (simp add: split_relation_def)
+
+(* auxiliary lemmas on assns *)
+(* simp? not sure if it always makes things more easy *)
+lemma list_assn_prod_map: "list_assn (A \<times>\<^sub>a B) xs ys = list_assn B (map snd xs) (map snd ys) * list_assn A (map fst xs) (map fst ys)"
+  apply(induct "(A \<times>\<^sub>a B)" xs ys rule: list_assn.induct)
+  apply(auto simp add: ab_semigroup_mult_class.mult.left_commute ent_star_mono star_aci(2) star_assoc)
+  done
+
+(* concrete *)
+lemma id_assn_list: "h \<Turnstile> list_assn id_assn (xs::'a list) ys \<Longrightarrow> xs = ys"
+  apply(induction "id_assn::('a \<Rightarrow> 'a \<Rightarrow> assn)" xs ys rule: list_assn.induct)
+  apply(auto simp add: less_Suc_eq_0_disj pure_def)
+  done
+
+
+lemma snd_map_help:
+  "x \<le> length tsi \<Longrightarrow>
+       (\<forall>j<x. snd (tsi ! j) = ((map snd tsi)!j))"
+  "x < length tsi \<Longrightarrow> snd (tsi!x) = ((map snd tsi)!x)"
+  by auto
+
+
+lemma split_ismeq: "((a::nat) \<le> b \<and> X) = ((a < b \<and> X) \<or> (a = b \<and> X))"
+  by auto
+
+lemma split_relation_map: "split_relation as (ls,rs) i \<Longrightarrow> split_relation (map f as) (map f ls, map f rs) i"
+  apply(induction as arbitrary: ls rs i)
+  apply(auto simp add: split_relation_def take_map drop_Cons')
+  apply (metis list.simps(9) take_map)
+  apply (simp add: drop_map)
+  done
+
+lemma split_relation_access: "\<lbrakk>split_relation as (ls,rs) i; rs = r#rrs\<rbrakk> \<Longrightarrow> as!i = r"
+  by (simp add: split_relation_alt)
+
+
+
+lemma index_to_elem_all: "(\<forall>j<length xs. P (xs!j)) = (\<forall>x \<in> set xs. P x)"
+  by (simp add: all_set_conv_nth)
+
+lemma index_to_elem: "n < length xs \<Longrightarrow> (\<forall>j<n. P (xs!j)) = (\<forall>x \<in> set (take n xs). P x)"
+  by (simp add: all_set_conv_nth)
+(* ----------------- *)
+
+definition split_half :: "('a::heap \<times> 'b::{heap}) pfarray \<Rightarrow> nat Heap"
+  where
+    "split_half a \<equiv> do {
+  l \<leftarrow> pfa_length a;
+  return (l div 2)
+}"
+
+lemma split_half_rule[sep_heap_rules]: "<
+    is_pfa c tsi a
+  * list_assn R ts tsi> 
+    split_half a
+  <\<lambda>i. 
+      is_pfa c tsi a
+    * list_assn R ts tsi
+    * \<up>(i = length ts div 2 \<and>  split_relation ts (BTree_Set.split_half ts) i)>"
+  unfolding split_half_def split_relation_def
+  apply(rule hoare_triple_preI)
+  apply(sep_auto dest!: list_assn_len mod_starD)
+  done
+
+locale imp_split = abs_split: BTree_Set.split split
+  for split::"('a btree \<times> 'a::{heap,default,linorder}) list \<Rightarrow> 'a \<Rightarrow> ('a btree \<times> 'a) list \<times> ('a btree \<times> 'a) list" +
+  fixes imp_split:: "('a btnode ref option \<times> 'a::{heap,default,linorder}) pfarray \<Rightarrow> 'a \<Rightarrow> nat Heap"
+  assumes imp_split_rule [sep_heap_rules]:"sorted_less (map snd ts) \<Longrightarrow>
+   <is_pfa c tsi (a,n)
+  * list_assn (btree_assn k \<times>\<^sub>a id_assn) ts tsi
+  * true> 
+    imp_split (a,n) p 
+  <\<lambda>i. 
+    is_pfa c tsi (a,n)
+    * list_assn (btree_assn k \<times>\<^sub>a id_assn) ts tsi
+    * \<up>(split_relation ts (split ts p) i)>\<^sub>t"
+begin
+
+partial_function (heap) isin :: "'a btnode ref option \<Rightarrow> 'a \<Rightarrow>  bool Heap"
+  where
+    "isin p x = 
+  (case p of 
+     None \<Rightarrow> return False |
+     (Some a) \<Rightarrow> do {
+       node \<leftarrow> !a;
+       i \<leftarrow> imp_split (kvs node) x;
+       tsl \<leftarrow> pfa_length (kvs node);
+       if i < tsl then do {
+         s \<leftarrow> pfa_get (kvs node) i;
+         let (sub,sep) = s in
+         if x = sep then
+           return True
+         else
+           isin sub x
+       } else
+           isin (last node) x
+    }
+)"
+
+
+lemma P_imp_Q_implies_P: "P \<Longrightarrow> (Q \<longrightarrow> P)"
+  by simp
+
+
+lemma  "sorted_less (inorder t) \<Longrightarrow>
+   <btree_assn k t ti * true>
+     isin ti x
+   <\<lambda>r. btree_assn k t ti * \<up>(abs_split.isin t x = r)>\<^sub>t"
+proof(induction t x arbitrary: ti rule: abs_split.isin.induct)
+  case (1 x)
+  then show ?case
+    apply(subst isin.simps)
+    apply (cases ti)
+    apply (auto simp add: return_cons_rule)
+    done
+next
+  case (2 ts t x)
+  then obtain ls rs where list_split[simp]: "split ts x = (ls,rs)"
+    by (cases "split ts x")
+  then show ?case
+  proof (cases rs)
+    (* NOTE: induction condition trivial here *)
+    case [simp]: Nil
+    show ?thesis
+      apply(subst isin.simps)
+      apply(sep_auto)
+      using "2.prems" sorted_inorder_separators apply blast
+      apply(auto simp add: split_relation_def dest!: sym[of "[]"] mod_starD list_assn_len)[]
+      apply(rule hoare_triple_preI)
+      apply(auto simp add: split_relation_def dest!: sym[of "[]"] mod_starD list_assn_len)[]
+      using 2(3) apply(sep_auto heap: "2.IH"(1)[of ls "[]"] simp add: sorted_wrt_append)
+      done
+  next
+    case [simp]: (Cons h rrs)
+    obtain sub sep where h_split[simp]: "h = (sub,sep)"
+      by (cases h)
+    show ?thesis
+    proof (cases "sep = x")
+      (* NOTE: no induction required here, only vacuous counter cases generated *)
+      case [simp]: True
+      then show ?thesis
+        apply(simp split: list.splits prod.splits)
+        apply(subst isin.simps)
+        using "2.prems" sorted_inorder_separators apply(sep_auto)
+        apply(rule hoare_triple_preI)
+        apply(auto simp add: split_relation_alt list_assn_append_Cons_left dest!: mod_starD list_assn_len)[]
+        apply(rule hoare_triple_preI)
+        apply(auto simp add: split_relation_def dest!: sym[of "[]"] mod_starD list_assn_len)[]
+        done
+    next
+      case [simp]: False
+      show ?thesis
+        apply(simp split: list.splits prod.splits)
+        apply safe
+        using False apply simp
+        apply(subst isin.simps)
+        using "2.prems" sorted_inorder_separators 
+          apply(sep_auto)
+          (*eliminate vacuous case*)
+        apply(auto simp add: split_relation_alt list_assn_append_Cons_left dest!:  mod_starD list_assn_len)[]
+          (* simplify towards induction step *)
+        apply(auto simp add: split_relation_alt list_assn_append_Cons_left dest!: mod_starD list_assn_len)[]
+
+(* NOTE show that z = (suba, sepa) *)
+        apply(rule norm_pre_ex_rule)+
+        apply(rule hoare_triple_preI)
+        subgoal for p tsi n ti xsi suba sepa zs1 z zs2 _
+          apply(subgoal_tac "z = (suba, sepa)", simp)
+          using 2(3) apply(sep_auto
+              heap:"2.IH"(2)[of ls rs h rrs sub sep]
+              simp add: sorted_wrt_append)
+          using list_split Cons h_split apply simp_all
+            (* proof that previous assumptions hold later *)
+          apply(rule P_imp_Q_implies_P)
+          apply(rule ent_ex_postI[where x="(tsi,n)"])
+          apply(rule ent_ex_postI[where x="ti"])
+          apply(rule ent_ex_postI[where x="(zs1 @ (suba, sepa) # zs2)"])
+          apply(rule ent_ex_postI[where x="zs1"])
+          apply(rule ent_ex_postI[where x="z"])
+          apply(rule ent_ex_postI[where x="zs2"])
+          apply sep_auto
+            (* prove subgoal_tac assumption *)
+          apply (metis (no_types, lifting) list_assn_aux_ineq_len list_assn_len nth_append_length star_false_left star_false_right)
+          done
+            (* eliminate last vacuous case *)
+        apply(rule hoare_triple_preI)
+        apply(auto simp add: split_relation_def dest!: mod_starD list_assn_len)[]
+        done
+    qed
+  qed
+qed
+
+
+
+datatype 'b btupi = 
+  T\<^sub>i "'b btnode ref option" |
+  Up\<^sub>i "'b btnode ref option" "'b" "'b btnode ref option"
+
+fun btupi_assn where
+  "btupi_assn k (abs_split.T\<^sub>i l) (T\<^sub>i li) =
+   btree_assn k l li" |
+  "btupi_assn k (abs_split.Up\<^sub>i l a r) (Up\<^sub>i li ai ri) =
+   btree_assn k l li * id_assn a ai * btree_assn k r ri" |
+  "btupi_assn _ _ _ = false"
+
+
+
+definition node\<^sub>i :: "nat \<Rightarrow> ('a btnode ref option \<times> 'a) pfarray \<Rightarrow> 'a btnode ref option \<Rightarrow> 'a btupi Heap" where
+  "node\<^sub>i k a ti \<equiv> do {
+    n \<leftarrow> pfa_length a;
+    if n \<le> 2*k then do {
+      a' \<leftarrow> pfa_shrink_cap (2*k) a;
+      l \<leftarrow> ref (Btnode a' ti);
+      return (T\<^sub>i (Some l))
+    }
+    else do {
+      b \<leftarrow> (pfa_empty (2*k) :: ('a btnode ref option \<times> 'a) pfarray Heap);
+      i \<leftarrow> split_half a;
+      m \<leftarrow> pfa_get a i;
+      b' \<leftarrow> pfa_drop a (i+1) b;
+      a' \<leftarrow> pfa_shrink i a;
+      a'' \<leftarrow> pfa_shrink_cap (2*k) a';
+      let (sub,sep) = m in do {
+        l \<leftarrow> ref (Btnode a'' sub);
+        r \<leftarrow> ref (Btnode b' ti);
+        return (Up\<^sub>i (Some l) sep (Some r))
+      }
+    }
+}"
+term Array.upd
+
+thm drop_eq_ConsD
+
+find_theorems "<emp>_<_>"
+
+
+
+declare abs_split.node\<^sub>i.simps [simp add]
+lemma node\<^sub>i_rule: assumes c_cap: "2*k \<le> c" "c \<le> 4*k+1"
+  shows "<is_pfa c tsi (a,n) * list_assn ((btree_assn k) \<times>\<^sub>a id_assn) ts tsi * btree_assn k t ti * true>
+  node\<^sub>i k (a,n) ti
+  <\<lambda>r. btupi_assn k (abs_split.node\<^sub>i k ts t) r >\<^sub>t"
+proof (cases "length ts \<le> 2*k")
+  case [simp]: True
+  then show ?thesis
+    apply(subst node\<^sub>i_def)
+    apply(rule hoare_triple_preI)
+    apply(sep_auto dest!: mod_starD list_assn_len)
+    apply(sep_auto simp add: is_pfa_def)[]
+    using c_cap apply(sep_auto simp add: is_pfa_def)[]
+    apply(sep_auto  dest!: mod_starD list_assn_len)[]
+    using True apply(sep_auto dest!: mod_starD list_assn_len)
+    done
+next
+  case [simp]: False
+  then obtain ls sub sep rs where
+    split_half_eq: "BTree_Set.split_half ts = (ls,(sub,sep)#rs)"
+    using node\<^sub>i_cases by blast
+  then show ?thesis
+    apply(subst node\<^sub>i_def)
+    apply(rule hoare_triple_preI)
+    apply(sep_auto dest!: mod_starD list_assn_len)
+    apply(sep_auto simp add:  split_relation_alt split_relation_length is_pfa_def dest!: mod_starD list_assn_len)
+
+    using False apply(sep_auto simp add: split_relation_alt )
+    using False  apply(sep_auto simp add: is_pfa_def)[]
+    apply(sep_auto)[]
+    apply(sep_auto simp add: is_pfa_def split_relation_alt)[]
+    using c_cap apply(sep_auto simp add: is_pfa_def)[]
+    apply(sep_auto)[]
+    using c_cap apply(sep_auto simp add: is_pfa_def)[]
+    using c_cap apply(simp)
+    apply(vcg)
+    apply(simp)
+    apply(rule impI)
+    subgoal for _ _ _ _ _ _ rsa subi ba rn lsi al ar _
+      thm ent_ex_postI
+      thm ent_ex_postI[where x="take (length tsi div 2) tsi"]
+        (* instantiate right hand side *)
+      apply(rule ent_ex_postI[where x="(rsa,rn)"])
+      apply(rule ent_ex_postI[where x="ti"])
+      apply(rule ent_ex_postI[where x="(drop (Suc (length tsi div 2)) tsi)"])
+      apply(rule ent_ex_postI[where x="lsi"])
+      apply(rule ent_ex_postI[where x="subi"])
+      apply(rule ent_ex_postI[where x="take (length tsi div 2) tsi"])
+        (* introduce equality between equality of split tsi/ts and original lists *)
+      apply(simp add: split_relation_alt)
+      apply(subgoal_tac "tsi =
+            take (length tsi div 2) tsi @ (subi, ba) # drop (Suc (length tsi div 2)) tsi")
+      apply(rule back_subst[where a="list_assn (btree_assn k \<times>\<^sub>a id_assn) ts (take (length tsi div 2) tsi @ (subi, ba) # (drop (Suc (length tsi div 2)) tsi))" and b="list_assn (btree_assn k \<times>\<^sub>a id_assn) ts tsi"])
+      apply(rule back_subst[where a="list_assn (btree_assn k \<times>\<^sub>a id_assn) (take (length tsi div 2) ts @ (sub, sep) # rs)" and b="list_assn (btree_assn k \<times>\<^sub>a id_assn) ts"])
+      apply(subst list_assn_aux_append_Cons)
+      apply sep_auto
+      apply sep_auto
+      apply simp
+      apply simp
+      apply(rule back_subst[where a="tsi ! (length tsi div 2)" and b="(subi, ba)"])
+      apply(rule id_take_nth_drop)
+      apply simp
+      apply simp
+      done
+    done
+qed
+declare abs_split.node\<^sub>i.simps [simp del]
+
+term Array.set
+
+partial_function (heap) ins :: "nat \<Rightarrow> 'a \<Rightarrow> 'a btnode ref option \<Rightarrow> 'a btupi Heap"
+  where
+    "ins k x p = (case p of
+  None \<Rightarrow> 
+    return (Up\<^sub>i None x None) |
+  (Some a) \<Rightarrow> do {
+    node \<leftarrow> !a;
+    i \<leftarrow> imp_split (kvs node) x;
+    tsl \<leftarrow> pfa_length (kvs node);
+    if i < tsl then do {
+      s \<leftarrow> pfa_get (kvs node) i;
+      let (sub,sep) = s in
+      if sep = x then
+        return (T\<^sub>i p)
+      else do {
+        r \<leftarrow> ins k x sub;
+        case r of 
+          (T\<^sub>i lp) \<Rightarrow> do {
+            pfa_set (kvs node) i (lp,sep);
+            return (T\<^sub>i p)
+          } |
+          (Up\<^sub>i lp x' rp) \<Rightarrow> do {
+            kvs' \<leftarrow> pfa_set (kvs node) i (rp,sep);
+            kvs'' \<leftarrow> pfa_insert_grow kvs' i (lp,x');
+            node\<^sub>i k kvs'' (last node)
+          }
+        }
+      }
+    else do {
+      r \<leftarrow> ins k x (last node);
+      case r of 
+        (T\<^sub>i lp) \<Rightarrow> do {
+          a := (Btnode (kvs node) lp);
+          return (T\<^sub>i p)
+        } |
+        (Up\<^sub>i lp x' rp) \<Rightarrow> do {
+          kvs' \<leftarrow> pfa_append_grow' (kvs node) (lp,x');
+          node\<^sub>i k kvs' rp
+        }
+    }
+  }
+)"
+
+
+(* this does not work anymore since we are inside a locale
+declare ins.simps[code]
+export_code ins checking SML Scala *)
+
+declare abs_split.node\<^sub>i.simps[simp del]
+
+lemma node\<^sub>i_rule_app: "\<lbrakk>2*k \<le> c; c \<le> 4*k+1\<rbrakk> \<Longrightarrow>
+<is_pfa c (tsi' @ [(li, ai)]) (aa, al) *
+   list_assn (btree_assn k \<times>\<^sub>a id_assn) ls tsi' *
+   btree_assn k l li *
+   id_assn a ai *
+   btree_assn k r ri *
+   true> node\<^sub>i k (aa, al) ri
+ <btupi_assn k (abs_split.node\<^sub>i k (ls @ [(l, a)]) r)>\<^sub>t"
+proof -
+  note node\<^sub>i_rule[of k c "(tsi' @ [(li, ai)])" aa al "(ls @ [(l, a)])" r ri]
+  moreover assume "2*k \<le> c" "c \<le> 4*k+1"
+  ultimately show ?thesis
+    by (simp add: mult.left_assoc)
+qed
+
+lemma node\<^sub>i_rule_ins2: "\<lbrakk>2*k \<le> c; c \<le> 4*k+1; length ls = length lsi\<rbrakk> \<Longrightarrow>
+ <is_pfa c (lsi @ (li, ai) # (ri,a'i) # rsi) (aa, al) *
+   list_assn (btree_assn k \<times>\<^sub>a id_assn) ls lsi *
+   btree_assn k l li *
+   id_assn a ai *
+   btree_assn k r ri *
+   id_assn a' a'i *
+   list_assn (btree_assn k \<times>\<^sub>a id_assn) rs rsi *
+   btree_assn k t ti *
+   true> node\<^sub>i k (aa, al)
+          ti <btupi_assn k (abs_split.node\<^sub>i k (ls @ (l, a) # (r,a') # rs) t)>\<^sub>t"
+proof -
+  assume [simp]: "2*k \<le> c" "c \<le> 4*k+1" "length ls = length lsi"
+  moreover note node\<^sub>i_rule[of k c "(lsi @ (li, ai) # (ri,a'i) # rsi)" aa al "(ls @ (l, a) # (r,a') # rs)" t ti]
+  ultimately show ?thesis
+    by (simp add: mult.left_assoc list_assn_aux_append_Cons)
+qed
+
+lemma ins_rule:
+  "sorted_less (inorder t) \<Longrightarrow> <btree_assn k t ti * true>
+  ins k x ti
+  <\<lambda>r. btupi_assn k (abs_split.ins k x t) r>\<^sub>t"
+proof (induction k x t arbitrary: ti rule: abs_split.ins.induct)
+  case (1 k x)
+  then show ?case
+    apply(subst ins.simps)
+    apply (sep_auto simp add: pure_app_eq)
+    done
+next
+  case (2 k x ts t)
+  obtain ls rrs where list_split: "split ts x = (ls,rrs)"
+    by (cases "split ts x")
+  have [simp]: "sorted_less (separators ts)"
+    using "2.prems" sorted_inorder_separators by simp
+  have [simp]: "sorted_less (inorder t)"
+    using "2.prems" sorted_inorder_induct_last by simp
+  show ?case
+  proof (cases rrs)
+    case Nil
+    then show ?thesis
+    proof (cases "abs_split.ins k x t")
+      case (T\<^sub>i a)
+      then show ?thesis
+        apply(subst ins.simps)
+        apply(sep_auto)
+        subgoal for p tsil tsin tti
+          using Nil list_split
+          by (simp add: Imperative_Loops.list_assn_aux_ineq_len split_relation_alt)
+        subgoal for p tsil tsin tti tsi' xb xaa xc sub sep
+          apply(rule hoare_triple_preI)
+          using Nil list_split
+          by (simp add: Imperative_Loops.list_assn_aux_ineq_len split_relation_alt)
+        subgoal for p tsil tsin tti tsi' xb xaa
+          thm "2.IH"(1)[of ls rrs tti]
+          using Nil list_split T\<^sub>i apply(sep_auto split!: list.splits simp add: split_relation_alt
+              heap add: "2.IH"(1)[of ls rrs tti])
+          subgoal for xi
+            apply(cases xi)
+            apply sep_auto
+            apply sep_auto
+            done
+          done
+        done
+    next
+      case (Up\<^sub>i l a r)
+      then show ?thesis
+        apply(subst ins.simps)
+        apply(sep_auto)
+        subgoal for p tsil tsin tti
+          using Nil list_split
+          by (simp add: Imperative_Loops.list_assn_aux_ineq_len split_relation_alt)                 
+        subgoal for p tsil tsin tti tsi' xb xaa xc sub sep
+          using Nil list_split 
+          by (simp add: Imperative_Loops.list_assn_aux_ineq_len split_relation_alt)
+        subgoal for p tsil tsin tti tsi' xb xaa
+          thm "2.IH"(1)[of ls rrs tti]
+          using Nil list_split Up\<^sub>i apply(sep_auto split!: list.splits 
+              simp add: split_relation_alt
+              heap add: "2.IH"(1)[of ls rrs tti])
+          subgoal for xi
+            apply(cases xi)
+            apply sep_auto
+            apply(sep_auto heap add: node\<^sub>i_rule_app)
+            done
+          done
+        done
+    qed
+  next
+    case (Cons a rs)
+    obtain sub sep where a_split: "a = (sub,sep)"
+      by (cases a)
+    then have [simp]: "sorted_less (inorder sub)"
+      using "2.prems" abs_split.split_axioms list_split Cons sorted_inorder_induct_subtree split_def
+      by fastforce
+    then show ?thesis
+    proof(cases "x = sep")
+      case True
+      show ?thesis
+        apply(subst ins.simps)
+        apply(sep_auto)
+        subgoal for p tsil tsin tti tsi j subi
+          using Cons list_split a_split True
+          by sep_auto
+        subgoal for p tsil tsin tti tsi j _ _ subi sepi
+          apply(rule hoare_triple_preI)
+          using Cons list_split a_split True
+          apply(subgoal_tac "sepi = sep")
+          apply (sep_auto simp add: split_relation_alt)
+          apply(sep_auto simp add: list_assn_prod_map dest!: mod_starD id_assn_list)
+          by (metis length_map snd_conv snd_map_help(2) split_relation_access)
+        subgoal for p tsil tsin tti tsi j
+          apply(rule hoare_triple_preI)
+          using Cons list_split
+          by (sep_auto simp add: split_relation_alt dest!: mod_starD list_assn_len)
+        done
+    next
+      case False
+      then show ?thesis
+      proof (cases "abs_split.ins k x sub")
+        case (T\<^sub>i a')
+        then show ?thesis
+          apply(auto simp add: Cons list_split a_split False)
+          using False apply simp
+          apply(subst ins.simps)
+          apply vcg
+          apply auto
+          apply(rule norm_pre_ex_rule)+
+            (* at this point, we want to introduce the split, and after that tease the
+  hoare triple assumptions out of the bracket, s.t. we don't split twice *)
+          apply vcg
+          apply sep_auto
+          using list_split Cons
+          apply(simp add: split_relation_alt list_assn_append_Cons_left)
+          apply (rule impI)
+          apply(rule norm_pre_ex_rule)+
+          apply(rule hoare_triple_preI)
+          apply sep_auto
+            (* discard wrong branch *)
+          subgoal for p tsil tsin ti zs1 subi sepi zs2 _ _ suba
+            apply(subgoal_tac "sepi  = x")
+            using list_split Cons a_split
+            apply(auto  dest!:  mod_starD )[]
+            apply(auto dest!:  mod_starD list_assn_len)[]
+            done
+              (* actual induction branch *)
+          subgoal for p tsil tsin ti zs1 subi sepi zs2 _ _ n z suba sepa
+            apply (cases a, simp)
+            apply(subgoal_tac "subi = suba", simp)
+            using list_split a_split T\<^sub>i False
+            apply (vcg heap: 2)
+            apply(auto split!: btupi.splits)
+              (* careful progression for manual value insertion *)
+            apply vcg
+            apply simp
+            apply vcg
+            apply simp
+            subgoal for a'i q r
+              apply(rule impI)
+              apply(simp add: list_assn_append_Cons_left)
+              apply(rule ent_ex_postI[where x="(tsil,tsin)"])
+              apply(rule ent_ex_postI[where x="ti"])
+              apply(rule ent_ex_postI[where x="(zs1 @ (a'i, sepi) # zs2)"])
+              apply(rule ent_ex_postI[where x="zs1"])
+              apply(rule ent_ex_postI[where x="(a'i,sep)"])
+              apply(rule ent_ex_postI[where x="zs2"])
+              apply sep_auto
+              apply (simp add: pure_app_eq)
+              apply(sep_auto dest!:  mod_starD list_assn_len)[]
+              done
+            apply (metis Imperative_Loops.list_assn_aux_ineq_len Pair_inject list_assn_len nth_append_length star_false_left star_false_right)
+            done
+          subgoal for p tsil tsin ti zs1 subi sepi zs2 _ _ suba
+            apply(auto dest!:  mod_starD list_assn_len)[]
+            done
+          done
+      next
+        case (Up\<^sub>i l w r)
+        then show ?thesis
+          apply(auto simp add: Cons list_split a_split False)
+          using False apply simp
+          apply(subst ins.simps)
+          apply vcg
+          apply auto
+          apply(rule norm_pre_ex_rule)+
+            (* at this point, we want to introduce the split, and after that tease the
+  hoare triple assumptions out of the bracket, s.t. we don't split twice *)
+          apply vcg
+          apply sep_auto
+          using list_split Cons
+          apply(simp add: split_relation_alt list_assn_append_Cons_left)
+          apply (rule impI)
+          apply(rule norm_pre_ex_rule)+
+          apply(rule hoare_triple_preI)
+          apply sep_auto
+            (* discard wrong branch *)
+          subgoal for p tsil tsin ti zs1 subi sepi zs2 _ _ suba
+            apply(subgoal_tac "sepi  = x")
+            using list_split Cons a_split
+            apply(auto  dest!:  mod_starD )[]
+            apply(auto dest!:  mod_starD list_assn_len)[]
+            done
+              (* actual induction branch *)
+          subgoal for p tsil tsin ti zs1 subi sepi zs2 _ _ n z suba sepa
+            apply(subgoal_tac "subi = suba", simp)
+            thm 2(2)[of ls rrs a rs sub sep]
+            using list_split a_split Cons Up\<^sub>i False
+            apply (sep_auto heap: 2(2))
+            apply(auto split!: btupi.splits)
+              (* careful progression for manual value insertion *)
+            apply vcg
+            apply simp
+            subgoal for x21 x22 x23 u
+              apply (cases u,simp)
+              thm pfa_insert_grow_rule[where ?l="((zs1 @ (suba, sepi) # zs2)[length ls := (x23, sepa)])"]
+              apply (sep_auto dest!: mod_starD list_assn_len heap: pfa_insert_grow_rule)
+              apply (simp add: is_pfa_def)[]
+              apply (metis le_less_linear length_append length_take less_not_refl min.absorb2 trans_less_add1)
+              apply(auto split: prod.splits  dest!: mod_starD list_assn_len)[]
+
+              apply (vcg heap: node\<^sub>i_rule_ins2)
+              apply simp
+              apply simp
+              apply simp
+              apply sep_auto
+              done
+            apply(auto dest!:  mod_starD list_assn_len)[]
+            done
+          subgoal for p tsil tsin ti zs1 subi sepi zs2 _ _ suba
+            apply(auto dest!:  mod_starD list_assn_len)[]
+            done
+          done
+      qed
+    qed
+  qed
+qed
+
+(*fun tree\<^sub>i::"'a up\<^sub>i \<Rightarrow> 'a btree" where
+  "tree\<^sub>i (T\<^sub>i sub) = sub" |
+  "tree\<^sub>i (Up\<^sub>i l a r) = (Node [(l,a)] r)" 
+
+fun insert::"nat \<Rightarrow> 'a \<Rightarrow> 'a btree \<Rightarrow> 'a btree" where
+  "insert k x t = tree\<^sub>i (ins k x t)"
+*)
+
+definition insert :: "nat \<Rightarrow> ('a::{heap,default,linorder}) \<Rightarrow> 'a btnode ref option \<Rightarrow> 'a btnode ref option Heap" where
+  "insert \<equiv> \<lambda>k x ti. do {
+  ti' \<leftarrow> ins k x ti;
+  case ti' of
+     T\<^sub>i sub \<Rightarrow> return sub |
+     Up\<^sub>i l a r \<Rightarrow> do {
+        kvs \<leftarrow> pfa_init (2*k) (l,a) 1;
+        t' \<leftarrow> ref (Btnode kvs r);
+        return (Some t')
+      }
+}"
+
+
+lemma insert'_rule:
+  assumes "k > 0" "sorted_less (inorder t)"
+  shows "<btree_assn k t ti * true>
+  insert k x ti
+  <\<lambda>r. btree_assn k (abs_split.insert k x t) r>\<^sub>t"
+  unfolding insert_def
+  apply(cases "abs_split.ins k x t")
+  apply(sep_auto split!: btupi.splits heap: ins_rule[OF assms(2)])
+  using assms
+  apply(vcg heap: ins_rule[OF assms(2)])
+  apply(simp split!: btupi.splits)
+  apply(vcg)
+  apply simp
+  apply simp
+  apply vcg
+  apply auto[]
+  subgoal for x21 x22 x23 x21a x22a x23a a b xa
+    apply(rule ent_ex_postI[where x="(a,b)"])
+    apply(rule ent_ex_postI[where x="x23a"])
+    apply(rule ent_ex_postI[where x="[(x21a, x22a)]"])
+    apply sep_auto
+    done
+  done
+
+
+
+(* rebalance middle tree gets a list of trees, an index pointing to
+the position of sub/sep and a last tree *)
+definition rebalance_middle_tree:: "nat \<Rightarrow> (('a::{default,heap,linorder}) btnode ref option \<times> 'a) pfarray \<Rightarrow> nat \<Rightarrow> 'a btnode ref option \<Rightarrow> 'a btnode Heap"
+  where
+    "rebalance_middle_tree \<equiv> \<lambda> k tsi i r_ti. (
+  case r_ti of
+  None \<Rightarrow> do {
+    return (Btnode tsi r_ti)
+  } |
+  Some p_t \<Rightarrow> do {
+      ti \<leftarrow> !p_t;
+      (r_sub,sep) \<leftarrow> pfa_get tsi i;
+      case r_sub of (Some p_sub) \<Rightarrow>  do {
+      sub \<leftarrow> !p_sub;
+      l_sub \<leftarrow> pfa_length (kvs sub);
+      l_ti \<leftarrow> pfa_length (kvs ti);
+      if l_sub \<ge> k \<and> l_ti \<ge> k then do {
+        return (Btnode tsi r_ti)
+      } else do {
+        l_tsi \<leftarrow> pfa_length tsi;
+        if l_tsi = (i+1) then do {
+          mts' \<leftarrow> pfa_append_extend_grow (kvs sub) (last sub,sep) (kvs ti);
+          res_node\<^sub>i \<leftarrow> node\<^sub>i k mts' (last ti);
+          case res_node\<^sub>i of
+            T\<^sub>i u \<Rightarrow> return (Btnode tsi u) |
+            Up\<^sub>i l a r \<Rightarrow> do {
+              tsi' \<leftarrow> pfa_append tsi (l,a);
+              return (Btnode tsi' r)
+            }
+        } else do {
+          (r_rsub,rsep) \<leftarrow> pfa_get tsi (i+1);
+          case r_rsub of Some p_rsub \<Rightarrow> do {
+            rsub \<leftarrow> !p_rsub;
+            mts' \<leftarrow> pfa_append_extend_grow (kvs sub) (last sub,sep) (kvs rsub);
+            res_node\<^sub>i \<leftarrow> node\<^sub>i k mts' (last rsub);
+            case res_node\<^sub>i of
+             T\<^sub>i u \<Rightarrow> do {
+              tsi' \<leftarrow> pfa_set tsi (i+1) (u,rsep);              
+              tsi'' \<leftarrow> pfa_delete tsi' i;
+              return (Btnode tsi'' r_ti)
+            } |
+             Up\<^sub>i l a r \<Rightarrow> do {
+              tsi' \<leftarrow> pfa_set tsi i (l,a);
+              tsi'' \<leftarrow> pfa_set tsi' (i+1) (r,rsep);
+              return (Btnode tsi'' r_ti)
+            }
+          }
+        }
+      }
+  }
+})
+"
+
+definition rebalance_last_tree:: "nat \<Rightarrow> (('a::{default,heap,linorder}) btnode ref option \<times> 'a) pfarray \<Rightarrow> 'a btnode ref option \<Rightarrow> 'a btnode Heap"
+  where
+    "rebalance_last_tree \<equiv> \<lambda>k tsi ti. do {
+   l_tsi \<leftarrow> pfa_length tsi;
+   rebalance_middle_tree k tsi (l_tsi-1) ti
+}"
+
+partial_function (heap) split_max ::"nat \<Rightarrow> ('a::{default,heap,linorder}) btnode ref option \<Rightarrow> ('a btnode ref option \<times> 'a) Heap"
+  where
+    "split_max k r_t = (case r_t of Some p_t \<Rightarrow> do {
+   t \<leftarrow> !p_t;
+   (case t of Btnode tsi r_ti \<Rightarrow>
+     case r_ti of None \<Rightarrow> do {
+      (sub,sep) \<leftarrow> pfa_last tsi;
+      tsi' \<leftarrow> pfa_butlast tsi;
+      p_t := Btnode tsi' sub;
+      return (Some p_t, sep)
+  } |
+    _ \<Rightarrow> do {
+      (sub,sep) \<leftarrow> split_max k r_ti;
+      p_t' \<leftarrow> rebalance_last_tree k tsi sub;
+      p_t := p_t';
+      return (Some p_t, sep)
+  })
+})
+"
+
+partial_function (heap) del ::"nat \<Rightarrow> 'a \<Rightarrow> ('a::{default,heap,linorder}) btnode ref option \<Rightarrow> 'a btnode ref option Heap"
+  where
+    "del k x ti = (case ti of None \<Rightarrow> return None |
+   Some p \<Rightarrow> do {
+   node \<leftarrow> !p;
+   i \<leftarrow> imp_split (kvs node) x;
+   tsl \<leftarrow> pfa_length (kvs node);
+   if i < tsl then do {
+     s \<leftarrow> pfa_get (kvs node) i;
+     let (sub,sep) = s in
+     if x \<noteq> sep then do {
+       sub' \<leftarrow> del k x sub;
+       kvs' \<leftarrow> pfa_set (kvs node) i (sub',sep);
+       node' \<leftarrow> rebalance_middle_tree k kvs' i (last node);
+       ti' \<leftarrow> ref node';
+       return (Some ti')
+      }
+     else if sub = None then do{
+       pfa_delete (kvs node) i;
+       return ti
+     }
+     else do {
+        sm \<leftarrow> split_max k sub;
+        kvs' \<leftarrow> pfa_set (kvs node) i sm;
+        node' \<leftarrow> rebalance_middle_tree k kvs' i (last node);
+        ti' \<leftarrow> ref node';
+        return (Some ti')
+     }
+   } else do {
+       t' \<leftarrow> del k x (last node);
+       node' \<leftarrow> rebalance_last_tree k (kvs node) t';
+       ti' \<leftarrow> ref node';
+       return (Some ti')
+    }
+})
+"
+
+partial_function (heap) reduce_root ::"('a::{default,heap,linorder}) btnode ref option \<Rightarrow> 'a btnode ref option Heap"
+  where
+"reduce_root ti = (case ti of
+  None \<Rightarrow> return None |
+  Some p_t \<Rightarrow> do {
+    node \<leftarrow> !p_t;
+    tsl \<leftarrow> pfa_length (kvs node);
+    case tsl of 0 \<Rightarrow> return (last node) |
+    _ \<Rightarrow> return ti
+})"
+
+partial_function (heap) delete ::"nat \<Rightarrow> 'a \<Rightarrow> ('a::{default,heap,linorder}) btnode ref option \<Rightarrow> 'a btnode ref option Heap"
+  where
+"delete k x ti = do {
+  ti' \<leftarrow> del k x ti;
+  reduce_root ti'
+}"
+
+end
+
+
 find_consts name: while
 
 term split
@@ -139,7 +940,7 @@ sorted_less xs \<Longrightarrow>
     moreover assume "sorted_less (take n l'a)"
     ultimately have "\<And>j. j < (aa+n)div 2 \<Longrightarrow> (take n l'a) ! j < (take n l'a) ! ((aa + n) div 2)"
       using
-        sorted_wrt_nth_less[where ?P="(<)" and ?xs="(take n l'a)" and ?j="((aa + n) div 2)"]
+        sorted_wrt_nth_less[where ?P="(<)" and xs="(take n l'a)" and ?j="((aa + n) div 2)"]
         a b "0" by auto
     moreover fix j assume "j < (aa+n) div 2"
     ultimately show "l'a ! j < p" using "0" b
@@ -158,7 +959,7 @@ sorted_less xs \<Longrightarrow>
     moreover assume "sorted_less (take n l'a)"
     ultimately have "\<And>j. j < (aa+b)div 2 \<Longrightarrow> (take n l'a) ! j < (take n l'a) ! ((aa + b) div 2)"
       using
-        sorted_wrt_nth_less[where ?P="(<)" and ?xs="(take n l'a)" and ?j="((aa + b) div 2)"]
+        sorted_wrt_nth_less[where ?P="(<)" and xs="(take n l'a)" and ?j="((aa + b) div 2)"]
         a b t0 by auto
     moreover fix j assume "j < (aa+b) div 2"
     ultimately show "l'a ! j < p" using t0 b
@@ -176,7 +977,7 @@ sorted_less xs \<Longrightarrow>
     assume t5: "j < (aa + n) div 2"
     have "(aa+n) div 2 < n" using t0 by linarith
     then have "(take n l'a) ! j < (take n l'a) ! ((aa + n) div 2)"
-      using t0 sorted_wrt_nth_less[where ?xs="take n l'a" and ?j="((aa + n) div 2)"]
+      using t0 sorted_wrt_nth_less[where xs="take n l'a" and ?j="((aa + n) div 2)"]
         t1 t4 t5 by auto
     then show ?thesis
       using \<open>(aa + n) div 2 < n\<close> t5 by auto
@@ -190,7 +991,7 @@ sorted_less xs \<Longrightarrow>
     assume t5: "j < (aa + b) div 2"
     have "(aa+b) div 2 < n" using t3 t0 by linarith
     then have "(take n l'a) ! j < (take n l'a) ! ((aa + b) div 2)"
-      using t0 sorted_wrt_nth_less[where ?xs="take n l'a" and ?j="((aa + b) div 2)"]
+      using t0 sorted_wrt_nth_less[where xs="take n l'a" and ?j="((aa + b) div 2)"]
         t1 t4 t5 by auto
     then show ?thesis
       using \<open>(aa + b) div 2 < n\<close> t5 by auto
@@ -280,8 +1081,6 @@ sorted_less (map snd xs) \<Longrightarrow>
 
 
 
-lemma split_ismeq: "((a::nat) \<le> b \<and> X) = ((a < b \<and> X) \<or> (a = b \<and> X))"
-  by auto
 
 
 definition "abs_split xs x = (takeWhile (\<lambda>(_,s). s<x) xs, dropWhile (\<lambda>(_,s). s<x) xs)"
@@ -296,34 +1095,13 @@ interpretation btree_abs_search: split abs_split
     by (metis case_prod_conv hd_dropWhile le_less_linear list.sel(1) list.simps(3))
   done
 
-definition "split_relation xs \<equiv> \<lambda>(as,bs) i. i \<le> length xs \<and> as = take i xs \<and> bs = drop i xs"
-
-lemma split_relation_alt: 
-  "split_relation as (ls,rs) i = (as = ls@rs \<and> i = length ls)"
-  by (auto simp add: split_relation_def)
 
 
 
-lemma split_relation_map: "split_relation as (ls,rs) i \<Longrightarrow> split_relation (map f as) (map f ls, map f rs) i"
-  apply(induction as arbitrary: ls rs i)
-  apply(auto simp add: split_relation_def take_map drop_Cons')
-  apply (metis list.simps(9) take_map)
-  apply (simp add: drop_map)
-  done
-
-lemma split_relation_access: "\<lbrakk>split_relation as (ls,rs) i; rs = r#rrs\<rbrakk> \<Longrightarrow> as!i = r"
-  by (simp add: split_relation_alt)
-
-
-
-lemma index_to_elem_all: "(\<forall>j<length xs. P (xs!j)) = (\<forall>x \<in> set xs. P x)"
-  by (simp add: all_set_conv_nth)
-
-lemma index_to_elem: "n < length xs \<Longrightarrow> (\<forall>j<n. P (xs!j)) = (\<forall>x \<in> set (take n xs). P x)"
-  by (simp add: all_set_conv_nth)
 
 lemma abs_split_full: "\<forall>(_,s) \<in> set xs. s < p \<Longrightarrow> abs_split xs p = (xs,[])"
   by (simp add: abs_split_def)
+
 
 lemma abs_split_split:
   assumes "n < length xs" 
@@ -336,8 +1114,6 @@ lemma abs_split_split:
 
 
 
-lemma split_relation_length: "split_relation xs (ls,rs) (length xs) = (ls = xs \<and> rs = [])"
-  by (simp add: split_relation_def)
 
 thm index_to_elem_all[of ts "\<lambda>x. snd x < p"]
 
@@ -346,27 +1122,11 @@ lemma list_assn_all: "h \<Turnstile> (list_assn (\<up>\<circ>\<circ>P) xs ys) \<
   apply(auto simp add: less_Suc_eq_0_disj)
   done
 
-(* simp? not sure if it always makes things more easy *)
-lemma list_assn_prod_map: "list_assn (A \<times>\<^sub>a B) xs ys = list_assn B (map snd xs) (map snd ys) * list_assn A (map fst xs) (map fst ys)"
-  apply(induct "(A \<times>\<^sub>a B)" xs ys rule: list_assn.induct)
-  apply(auto simp add: ab_semigroup_mult_class.mult.left_commute ent_star_mono star_aci(2) star_assoc)
-  done
 
 find_theorems Id
 
 
-(* concrete *)
-lemma id_assn_list: "h \<Turnstile> list_assn id_assn (xs::'a list) ys \<Longrightarrow> xs = ys"
-  apply(induction "id_assn::('a \<Rightarrow> 'a \<Rightarrow> assn)" xs ys rule: list_assn.induct)
-  apply(auto simp add: less_Suc_eq_0_disj pure_def)
-  done
 
-
-lemma snd_map_help:
-  "x \<le> length tsi \<Longrightarrow>
-       (\<forall>j<x. snd (tsi ! j) = ((map snd tsi)!j))"
-  "x < length tsi \<Longrightarrow> snd (tsi!x) = ((map snd tsi)!x)"
-  by auto
 
 (* new, added for the "interesting part" *)
 
@@ -558,1153 +1318,80 @@ sorted_less (map snd ts) \<Longrightarrow> <
   apply(auto dest!: mod_starD id_assn_list simp add: list_assn_prod_map)
   done
 
-locale imp_split = abs_split: BTree_Set.split split
-  for split::"('a btree \<times> 'a::{heap,linorder}) list \<Rightarrow> 'a \<Rightarrow> ('a btree \<times> 'a) list \<times> ('a btree \<times> 'a) list" +
-  fixes imp_split:: "('a btnode ref option \<times> 'a::{heap,linorder}) pfarray \<Rightarrow> 'a \<Rightarrow> nat Heap"
-  assumes imp_split_rule [sep_heap_rules]:"sorted_less (map snd ts) \<Longrightarrow>
-   <is_pfa c tsi (a,n)
-  * list_assn (btree_assn k \<times>\<^sub>a id_assn) ts tsi
-  * true> 
-    imp_split (a,n) p 
-  <\<lambda>i. 
-    is_pfa c tsi (a,n)
-    * list_assn (btree_assn k \<times>\<^sub>a id_assn) ts tsi
-    * \<up>(split_relation ts (abs_split ts p) i)>\<^sub>t"
-begin
 
-partial_function (heap) imp_isin :: "'a btnode ref option \<Rightarrow> 'a \<Rightarrow>  bool Heap"
-  where
-    "imp_isin p x = 
-  (case p of 
-     None \<Rightarrow> return False |
-     (Some a) \<Rightarrow> do {
-       node \<leftarrow> !a;
-       i \<leftarrow> imp_split (kvs node) x;
-       tsl \<leftarrow> pfa_length (kvs node);
-       if i < tsl then do {
-         s \<leftarrow> pfa_get (kvs node) i;
-         let (sub,sep) = s in
-         if x = sep then
-           return True
-         else
-           imp_isin sub x
-       } else
-           imp_isin (last node) x
-    }
-)"
-
-
-lemma P_imp_Q_implies_P: "P \<Longrightarrow> (Q \<longrightarrow> P)"
-  by simp
-
-lemma  "sorted_less (inorder t) \<Longrightarrow>
-   <btree_assn k t ti * true>
-     imp_isin ti x
-   <\<lambda>r. btree_assn k t ti * \<up>(abs_split.isin t x = r)>\<^sub>t"
-proof(induction t x arbitrary: ti rule: abs_split.isin.induct)
-  case (1 x)
-  then show ?case
-    apply(subst imp_isin.simps)
-    apply (cases ti)
-    apply (auto simp add: return_cons_rule)
-    done
-next
-  case (2 ts t x)
-  then obtain ls rs where list_split[simp]: "abs_split ts x = (ls,rs)"
-    by (cases "abs_split ts x")
-  then show ?case
-  proof (cases rs)
-    (* NOTE: induction condition trivial here *)
-    case [simp]: Nil
-    show ?thesis
-      apply(subst imp_isin.simps)
-      apply(sep_auto)
-      apply(auto simp add: split_relation_def dest!: sym[of "[]"] mod_starD list_assn_len)[]
-      apply(rule hoare_triple_preI)
-      apply(auto simp add: split_relation_def dest!: sym[of "[]"] mod_starD list_assn_len)[]
-      using 2(3) apply(sep_auto heap: "2.IH"(1)[of ls "[]"] simp add: sorted_wrt_append)
-      done
-  next
-    case [simp]: (Cons h rrs)
-    obtain sub sep where h_split[simp]: "h = (sub,sep)"
-      by (cases h)
-    show ?thesis
-    proof (cases "sep = x")
-      (* NOTE: no induction required here, only vacuous counter cases generated *)
-      case [simp]: True
-      then show ?thesis
-        apply(simp split: list.splits prod.splits)
-        apply(subst isin.simps)
-        apply(sep_auto heap: bin_split_imp_abs_split)
-        apply(rule hoare_triple_preI)
-        apply(auto simp add: split_relation_alt list_assn_append_Cons_left dest!: mod_starD list_assn_len)[]
-        apply(rule hoare_triple_preI)
-        apply(auto simp add: split_relation_def dest!: sym[of "[]"] mod_starD list_assn_len)[]
-        done
-    next
-      case [simp]: False
-      show ?thesis
-        apply(simp split: list.splits prod.splits)
-        apply safe
-        using False apply simp
-        apply(subst isin.simps)
-        apply(sep_auto heap: bin_split_imp_abs_split)
-          (*eliminate vacuous case*)
-        apply(auto simp add: split_relation_alt list_assn_append_Cons_left dest!:  mod_starD list_assn_len)[]
-          (* simplify towards induction step *)
-        apply(auto simp add: split_relation_alt list_assn_append_Cons_left dest!: mod_starD list_assn_len)[]
-
-(* NOTE show that z = (suba, sepa) *)
-        apply(rule norm_pre_ex_rule)+
-        apply(rule hoare_triple_preI)
-        subgoal for p tsi n ti xsi suba sepa zs1 z zs2 _
-          apply(subgoal_tac "z = (suba, sepa)", simp)
-          using 2(3) apply(sep_auto heap:"2.IH"(2)[of ls rs h rrs sub sep] simp add: sorted_wrt_append)
-          using list_split Cons h_split apply simp_all
-            (* proof that previous assumptions hold later *)
-          apply(rule P_imp_Q_implies_P)
-          apply(rule ent_ex_postI[where ?x="(tsi,n)"])
-          apply(rule ent_ex_postI[where ?x="ti"])
-          apply(rule ent_ex_postI[where ?x="(zs1 @ (suba, sepa) # zs2)"])
-          apply(rule ent_ex_postI[where ?x="zs1"])
-          apply(rule ent_ex_postI[where ?x="z"])
-          apply(rule ent_ex_postI[where ?x="zs2"])
-          apply sep_auto
-            (* prove subgoal_tac assumption *)
-          apply (metis (no_types, lifting) list_assn_aux_ineq_len list_assn_len nth_append_length star_false_left star_false_right)
-          done
-            (* eliminate last vacuous case *)
-        apply(rule hoare_triple_preI)
-        apply(auto simp add: split_relation_def dest!: mod_starD list_assn_len)[]
-        done
-    qed
-  qed
-qed
-
-
-
-definition split_half :: "('a::heap \<times> 'b::{heap}) pfarray \<Rightarrow> nat Heap"
-  where
-    "split_half a \<equiv> do {
-  l \<leftarrow> pfa_length a;
-  return (l div 2)
-}"
-
-lemma split_half_rule[sep_heap_rules]: "<
-    is_pfa c tsi a
-  * list_assn R ts tsi> 
-    split_half a
-  <\<lambda>i. 
-      is_pfa c tsi a
-    * list_assn R ts tsi
-    * \<up>(i = length ts div 2 \<and>  split_relation ts (BTree_Set.split_half ts) i)>"
-  unfolding split_half_def split_relation_def
-  apply(rule hoare_triple_preI)
-  apply(sep_auto dest!: list_assn_len mod_starD)
+interpretation btree_linear_imp_split: imp_split abs_split lin_split
+  apply unfold_locales
+  apply(sep_auto heap: lin_split_imp_abs_split)
   done
 
-datatype 'a btupi = 
-  T\<^sub>i "'a btnode ref option" |
-  Up\<^sub>i "'a btnode ref option" "'a" "'a btnode ref option"
+definition [code del]: "linear_imp_insert = imp_split.insert lin_split"
 
-fun btupi_assn where
-  "btupi_assn k (btree_abs_search.T\<^sub>i l) (T\<^sub>i li) =
-   btree_assn k l li" |
-  "btupi_assn k (btree_abs_search.Up\<^sub>i l a r) (Up\<^sub>i li ai ri) =
-   btree_assn k l li * id_assn a ai * btree_assn k r ri" |
-  "btupi_assn _ _ _ = false"
+export_code linear_imp_insert checking SML Scala
 
+(* obtaining actual code turns out to be slightly more difficult
+  due to the use of locales *)
 
-
-definition node\<^sub>i :: "nat \<Rightarrow> (('a::{default,heap}) btnode ref option \<times> 'a) pfarray \<Rightarrow> 'a btnode ref option \<Rightarrow> 'a btupi Heap" where
-  "node\<^sub>i k a ti \<equiv> do {
-    n \<leftarrow> pfa_length a;
-    if n \<le> 2*k then do {
-      a' \<leftarrow> pfa_shrink_cap (2*k) a;
-      l \<leftarrow> ref (Btnode a' ti);
-      return (T\<^sub>i (Some l))
-    }
-    else do {
-      b \<leftarrow> (pfa_empty (2*k) :: ('a btnode ref option \<times> 'a) pfarray Heap);
-      i \<leftarrow> split_half a;
-      m \<leftarrow> pfa_get a i;
-      b' \<leftarrow> pfa_drop a (i+1) b;
-      a' \<leftarrow> pfa_shrink i a;
-      a'' \<leftarrow> pfa_shrink_cap (2*k) a';
-      let (sub,sep) = m in do {
-        l \<leftarrow> ref (Btnode a'' sub);
-        r \<leftarrow> ref (Btnode b' ti);
-        return (Up\<^sub>i (Some l) sep (Some r))
-      }
-    }
-}"
-term Array.upd
-
-thm drop_eq_ConsD
-
-find_theorems "<emp>_<_>"
-
-
-
-
-lemma node\<^sub>i_rule: assumes c_cap: "2*k \<le> c" "c \<le> 4*k+1"
-  shows "<is_pfa c tsi (a,n) * list_assn ((btree_assn k) \<times>\<^sub>a id_assn) ts tsi * btree_assn k t ti * true>
-  node\<^sub>i k (a,n) ti
-  <\<lambda>r. btupi_assn k (btree_abs_search.node\<^sub>i k ts t) r >\<^sub>t"
-proof (cases "length ts \<le> 2*k")
-  case [simp]: True
-  then show ?thesis
-    apply(subst node\<^sub>i_def)
-    apply(rule hoare_triple_preI)
-    apply(sep_auto dest!: mod_starD list_assn_len)
-    apply(sep_auto simp add: is_pfa_def)[]
-    using c_cap apply(sep_auto simp add: is_pfa_def)[]
-    apply(sep_auto  dest!: mod_starD list_assn_len)[]
-    using True apply(sep_auto dest!: mod_starD list_assn_len)
-    done
-next
-  case [simp]: False
-  then obtain ls sub sep rs where
-    split_half_eq: "BTree_Set.split_half ts = (ls,(sub,sep)#rs)"
-    using node\<^sub>i_cases by blast
-  then show ?thesis
-    apply(subst node\<^sub>i_def)
-    apply(rule hoare_triple_preI)
-    apply(sep_auto dest!: mod_starD list_assn_len)
-    apply(sep_auto simp add:  split_relation_alt split_relation_length is_pfa_def dest!: mod_starD list_assn_len)
-
-    using False apply(sep_auto simp add: split_relation_alt )
-    using False  apply(sep_auto simp add: is_pfa_def)[]
-    apply(sep_auto)[]
-    apply(sep_auto simp add: is_pfa_def split_relation_alt)[]
-    using c_cap apply(sep_auto simp add: is_pfa_def)[]
-    apply(sep_auto)[]
-    using c_cap apply(sep_auto simp add: is_pfa_def)[]
-    using c_cap apply(simp)
-    apply(vcg)
-    apply(simp)
-    apply(rule impI)
-    subgoal for _ _ _ _ _ _ rsa subi ba rn lsi al ar _
-      thm ent_ex_postI
-      thm ent_ex_postI[where ?x="take (length tsi div 2) tsi"]
-        (* instantiate right hand side *)
-      apply(rule ent_ex_postI[where ?x="(rsa,rn)"])
-      apply(rule ent_ex_postI[where ?x="ti"])
-      apply(rule ent_ex_postI[where ?x="(drop (Suc (length tsi div 2)) tsi)"])
-      apply(rule ent_ex_postI[where ?x="lsi"])
-      apply(rule ent_ex_postI[where ?x="subi"])
-      apply(rule ent_ex_postI[where ?x="take (length tsi div 2) tsi"])
-        (* introduce equality between equality of split tsi/ts and original lists *)
-      apply(simp add: split_relation_alt)
-      apply(subgoal_tac "tsi =
-            take (length tsi div 2) tsi @ (subi, ba) # drop (Suc (length tsi div 2)) tsi")
-      apply(rule back_subst[where a="list_assn (btree_assn k \<times>\<^sub>a id_assn) ts (take (length tsi div 2) tsi @ (subi, ba) # (drop (Suc (length tsi div 2)) tsi))" and b="list_assn (btree_assn k \<times>\<^sub>a id_assn) ts tsi"])
-      apply(rule back_subst[where a="list_assn (btree_assn k \<times>\<^sub>a id_assn) (take (length tsi div 2) ts @ (sub, sep) # rs)" and b="list_assn (btree_assn k \<times>\<^sub>a id_assn) ts"])
-      apply(subst list_assn_aux_append_Cons)
-      apply sep_auto
-      apply sep_auto
-      apply simp
-      apply simp
-      apply(rule back_subst[where a="tsi ! (length tsi div 2)" and b="(subi, ba)"])
-      apply(rule id_take_nth_drop)
-      apply simp
-      apply simp
-      done
-    done
-qed
-
-term Array.set
-
-partial_function (heap) ins :: "nat \<Rightarrow> 'a \<Rightarrow> ('a::{heap,linorder,default}) btnode ref option \<Rightarrow> 'a btupi Heap"
-  where
-    "ins k x p = (case p of
-  None \<Rightarrow> 
-    return (Up\<^sub>i None x None) |
-  (Some a) \<Rightarrow> do {
-    node \<leftarrow> !a;
-    i \<leftarrow> lin_split (kvs node) x;
-    tsl \<leftarrow> pfa_length (kvs node);
-    if i < tsl then do {
-      s \<leftarrow> pfa_get (kvs node) i;
-      let (sub,sep) = s in
-      if sep = x then
-        return (T\<^sub>i p)
-      else do {
-        r \<leftarrow> ins k x sub;
-        case r of 
-          (T\<^sub>i lp) \<Rightarrow> do {
-            pfa_set (kvs node) i (lp,sep);
-            return (T\<^sub>i p)
-          } |
-          (Up\<^sub>i lp x' rp) \<Rightarrow> do {
-            kvs' \<leftarrow> pfa_set (kvs node) i (rp,sep);
-            kvs'' \<leftarrow> pfa_insert_grow kvs' i (lp,x');
-            node\<^sub>i k kvs'' (last node)
-          }
-        }
-      }
-    else do {
-      r \<leftarrow> ins k x (last node);
-      case r of 
-        (T\<^sub>i lp) \<Rightarrow> do {
-          a := (Btnode (kvs node) lp);
-          return (T\<^sub>i p)
-        } |
-        (Up\<^sub>i lp x' rp) \<Rightarrow> do {
-          kvs' \<leftarrow> pfa_append_grow' (kvs node) (lp,x');
-          node\<^sub>i k kvs' rp
-        }
-    }
-  }
-)"
-
-declare ins.simps[code]
-export_code ins checking SML Scala
-
-declare btree_abs_search.node\<^sub>i.simps[simp del]
-
-
-lemma node\<^sub>i_rule_app: "\<lbrakk>2*k \<le> c; c \<le> 4*k+1\<rbrakk> \<Longrightarrow>
-<is_pfa c (tsi' @ [(li, ai)]) (aa, al) *
-   list_assn (btree_assn k \<times>\<^sub>a id_assn) ls tsi' *
-   btree_assn k l li *
-   id_assn a ai *
-   btree_assn k r ri *
-   true> node\<^sub>i k (aa, al) ri
- <btupi_assn k (btree_abs_search.node\<^sub>i k (ls @ [(l, a)]) r)>\<^sub>t"
-proof -
-  note node\<^sub>i_rule[of k c "(tsi' @ [(li, ai)])" aa al "(ls @ [(l, a)])" r ri]
-  moreover assume "2*k \<le> c" "c \<le> 4*k+1"
-  ultimately show ?thesis
-    by (simp add: mult.left_assoc)
-qed
-
-lemma node\<^sub>i_rule_ins2: "\<lbrakk>2*k \<le> c; c \<le> 4*k+1; length ls = length lsi\<rbrakk> \<Longrightarrow>
- <is_pfa c (lsi @ (li, ai) # (ri,a'i) # rsi) (aa, al) *
-   list_assn (btree_assn k \<times>\<^sub>a id_assn) ls lsi *
-   btree_assn k l li *
-   id_assn a ai *
-   btree_assn k r ri *
-   id_assn a' a'i *
-   list_assn (btree_assn k \<times>\<^sub>a id_assn) rs rsi *
-   btree_assn k t ti *
-   true> node\<^sub>i k (aa, al)
-          ti <btupi_assn k (btree_abs_search.node\<^sub>i k (ls @ (l, a) # (r,a') # rs) t)>\<^sub>t"
-proof -
-  assume [simp]: "2*k \<le> c" "c \<le> 4*k+1" "length ls = length lsi"
-  moreover note node\<^sub>i_rule[of k c "(lsi @ (li, ai) # (ri,a'i) # rsi)" aa al "(ls @ (l, a) # (r,a') # rs)" t ti]
-  ultimately show ?thesis
-    by (simp add: mult.left_assoc list_assn_aux_append_Cons)
-qed
-
-
-lemma ins_rule:
-  shows "<btree_assn k t ti * true>
-  ins k x ti
-  <\<lambda>r. btupi_assn k (btree_abs_search.ins k x t) r>\<^sub>t"
-proof (induction k x t arbitrary: ti rule: btree_abs_search.ins.induct)
-  case (1 k x)
-  then show ?case
-    apply(subst ins.simps)
-    apply (sep_auto simp add: pure_app_eq)
-    done
-next
-  case (2 k x ts t)
-  then obtain ls rrs where list_split: "abs_split ts x = (ls,rrs)"
-    by (cases "abs_split ts x")
-  then show ?case
-  proof (cases rrs)
-    case Nil
-    then show ?thesis
-    proof (cases "btree_abs_search.ins k x t")
-      case (T\<^sub>i a)
-      then show ?thesis
-        apply(subst ins.simps)
-        apply(sep_auto heap: lin_split_imp_abs_split)
-        subgoal for p tsil tsin tti
-          using Nil list_split
-          by (simp add: Imperative_Loops.list_assn_aux_ineq_len split_relation_alt)
-        subgoal for p tsil tsin tti tsi' xb xaa xc sub sep
-          apply(rule hoare_triple_preI)
-          using Nil list_split
-          by (simp add: Imperative_Loops.list_assn_aux_ineq_len split_relation_alt)
-        subgoal for p tsil tsin tti tsi' xb xaa
-          thm "2.IH"(1)[of ls rrs tti]
-          using Nil list_split T\<^sub>i apply(sep_auto split!: list.splits simp add: split_relation_alt
-              heap add: "2.IH"(1)[of ls rrs tti])
-          subgoal for xi
-            apply(cases xi)
-            apply sep_auto
-            apply sep_auto
-            done
-          done
-        done
-    next
-      case (Up\<^sub>i l a r)
-      then show ?thesis
-        apply(subst ins.simps)
-        apply(sep_auto heap: lin_split_imp_abs_split)
-        subgoal for p tsil tsin tti
-          using Nil list_split
-          by (simp add: Imperative_Loops.list_assn_aux_ineq_len split_relation_alt)                 
-        subgoal for p tsil tsin tti tsi' xb xaa xc sub sep
-          using Nil list_split 
-          by (simp add: Imperative_Loops.list_assn_aux_ineq_len split_relation_alt)
-        subgoal for p tsil tsin tti tsi' xb xaa
-          thm "2.IH"(1)[of ls rrs tti]
-          using Nil list_split Up\<^sub>i apply(sep_auto split!: list.splits simp add: split_relation_alt
-              heap add: "2.IH"(1)[of ls rrs tti])
-          subgoal for xi
-            apply(cases xi)
-            apply sep_auto
-            apply(sep_auto heap add: node\<^sub>i_rule_app)
-            done
-          done
-        done
-    qed
-  next
-    case (Cons a rs)
-    obtain sub sep where a_split: "a = (sub,sep)"
-      by (cases a)
-    then show ?thesis
-    proof(cases "x = sep")
-      case True
-      show ?thesis
-        apply(subst ins.simps)
-        apply(sep_auto heap: lin_split_imp_abs_split)
-        subgoal for p tsil tsin tti tsi j subi
-          using Cons list_split a_split True
-          by sep_auto
-        subgoal for p tsil tsin tti tsi j _ _ subi sepi
-          apply(rule hoare_triple_preI)
-          using Cons list_split a_split True
-          apply(subgoal_tac "sepi = sep")
-          apply (sep_auto simp add: split_relation_alt)
-          apply(sep_auto simp add: list_assn_prod_map dest!: mod_starD id_assn_list)
-          by (metis length_map snd_conv snd_map_help(2) split_relation_access)
-        subgoal for p tsil tsin tti tsi j
-          apply(rule hoare_triple_preI)
-          using Cons list_split
-          by (sep_auto simp add: split_relation_alt dest!: mod_starD list_assn_len)
-        done
-    next
-      case False
-      then show ?thesis
-      proof (cases "btree_abs_search.ins k x sub")
-        case (T\<^sub>i a')
-        then show ?thesis
-          apply(auto simp add: Cons list_split a_split False)
-          using False apply simp
-          apply(subst ins.simps)
-          apply vcg
-          apply auto
-          apply(rule norm_pre_ex_rule)+
-            (* at this point, we want to introduce the split, and after that tease the
-  hoare triple assumptions out of the bracket, s.t. we don't split twice *)
-          apply vcg
-          apply sep_auto
-          using list_split Cons
-          apply(simp add: split_relation_alt list_assn_append_Cons_left)
-          apply (rule impI)
-          apply(rule norm_pre_ex_rule)+
-          apply(rule hoare_triple_preI)
-          apply sep_auto
-            (* discard wrong branch *)
-          subgoal for p tsil tsin ti zs1 subi sepi zs2 _ _ suba
-            apply(subgoal_tac "sepi  = x")
-            using list_split Cons a_split
-            apply(auto  dest!:  mod_starD )[]
-            apply(auto dest!:  mod_starD list_assn_len)[]
-            done
-              (* actual induction branch *)
-          subgoal for p tsil tsin ti zs1 subi sepi zs2 _ _ n z suba sepa
-            apply (cases a, simp)
-            apply(subgoal_tac "subi = suba", simp)
-            using list_split a_split T\<^sub>i False
-            apply (vcg heap: 2)
-            apply(auto split!: btupi.splits)
-              (* careful progression for manual value insertion *)
-            apply vcg
-            apply simp
-            apply vcg
-            apply simp
-            subgoal for a'i q r
-              apply(rule impI)
-              apply(simp add: list_assn_append_Cons_left)
-              apply(rule ent_ex_postI[where ?x="(tsil,tsin)"])
-              apply(rule ent_ex_postI[where ?x="ti"])
-              apply(rule ent_ex_postI[where ?x="(zs1 @ (a'i, sepi) # zs2)"])
-              apply(rule ent_ex_postI[where ?x="zs1"])
-              apply(rule ent_ex_postI[where ?x="(a'i,sep)"])
-              apply(rule ent_ex_postI[where ?x="zs2"])
-              apply sep_auto
-              apply (simp add: pure_app_eq)
-              apply(sep_auto dest!:  mod_starD list_assn_len)[]
-              done
-            apply (metis Imperative_Loops.list_assn_aux_ineq_len Pair_inject list_assn_len nth_append_length star_false_left star_false_right)
-            done
-          subgoal for p tsil tsin ti zs1 subi sepi zs2 _ _ suba
-            apply(auto dest!:  mod_starD list_assn_len)[]
-            done
-          done
-      next
-        case (Up\<^sub>i l w r)
-        then show ?thesis
-          apply(auto simp add: Cons list_split a_split False)
-          using False apply simp
-          apply(subst ins.simps)
-          apply vcg
-          apply auto
-          apply(rule norm_pre_ex_rule)+
-            (* at this point, we want to introduce the split, and after that tease the
-  hoare triple assumptions out of the bracket, s.t. we don't split twice *)
-          apply vcg
-          apply sep_auto
-          using list_split Cons
-          apply(simp add: split_relation_alt list_assn_append_Cons_left)
-          apply (rule impI)
-          apply(rule norm_pre_ex_rule)+
-          apply(rule hoare_triple_preI)
-          apply sep_auto
-            (* discard wrong branch *)
-          subgoal for p tsil tsin ti zs1 subi sepi zs2 _ _ suba
-            apply(subgoal_tac "sepi  = x")
-            using list_split Cons a_split
-            apply(auto  dest!:  mod_starD )[]
-            apply(auto dest!:  mod_starD list_assn_len)[]
-            done
-              (* actual induction branch *)
-          subgoal for p tsil tsin ti zs1 subi sepi zs2 _ _ n z suba sepa
-            apply(subgoal_tac "subi = suba", simp)
-            thm 2(2)[of ls rrs a rs sub sep]
-            using list_split a_split Cons Up\<^sub>i False
-            apply (sep_auto heap: 2(2))
-            apply(auto split!: btupi.splits)
-              (* careful progression for manual value insertion *)
-            apply vcg
-            apply simp
-            subgoal for x21 x22 x23 u
-              apply (cases u,simp)
-              thm pfa_insert_grow_rule[where ?l="((zs1 @ (suba, sepi) # zs2)[length ls := (x23, sepa)])"]
-              apply (sep_auto dest!: mod_starD list_assn_len heap: pfa_insert_grow_rule)
-              apply (simp add: is_pfa_def)[]
-              apply (metis le_less_linear length_append length_take less_not_refl min.absorb2 trans_less_add1)
-              apply(auto split: prod.splits  dest!: mod_starD list_assn_len)[]
-
-              apply (vcg heap: node\<^sub>i_rule_ins2)
-              apply simp
-              apply simp
-              apply simp
-              apply sep_auto
-              done
-            apply(auto dest!:  mod_starD list_assn_len)[]
-            done
-          subgoal for p tsil tsin ti zs1 subi sepi zs2 _ _ suba
-            apply(auto dest!:  mod_starD list_assn_len)[]
-            done
-          done
-      qed
-    qed
-  qed
-qed
-
-declare btree_abs_search.ins.simps[simp del]
-
-(*fun tree\<^sub>i::"'a up\<^sub>i \<Rightarrow> 'a btree" where
-  "tree\<^sub>i (T\<^sub>i sub) = sub" |
-  "tree\<^sub>i (Up\<^sub>i l a r) = (Node [(l,a)] r)" 
-
-fun insert::"nat \<Rightarrow> 'a \<Rightarrow> 'a btree \<Rightarrow> 'a btree" where
-  "insert k x t = tree\<^sub>i (ins k x t)"
-*)
-
-definition insert :: "nat \<Rightarrow> ('a::{heap,default,linorder}) \<Rightarrow> 'a btnode ref option \<Rightarrow> 'a btnode ref option Heap" where
-  "insert \<equiv> \<lambda>k x ti. do {
-  ti' \<leftarrow> ins k x ti;
-  case ti' of
-     T\<^sub>i sub \<Rightarrow> return sub |
-     Up\<^sub>i l a r \<Rightarrow> do {
-        kvs \<leftarrow> pfa_init (2*k) (l,a) 1;
-        t' \<leftarrow> ref (Btnode kvs r);
-        return (Some t')
-      }
-}"
-
-lemma insert_rule:
-  assumes "k > 0"
-  shows "<btree_assn k t ti * true>
-  insert k x ti
-  <\<lambda>r. btree_assn k (btree_abs_search.insert k x t) r>\<^sub>t"
-  unfolding insert_def
-  apply(cases "btree_abs_search.ins k x t")
-  apply(sep_auto split!: btupi.splits heap: ins_rule)
-  using assms
-  apply(vcg heap: ins_rule)
-  apply(simp split!: btupi.splits)
-  apply(vcg)
-  apply simp
-  apply simp
-  apply vcg
-  apply auto[]
-  subgoal for x21 x22 x23 x21a x22a x23a a b xa
-    apply(rule ent_ex_postI[where ?x="(a,b)"])
-    apply(rule ent_ex_postI[where ?x="x23a"])
-    apply(rule ent_ex_postI[where ?x="[(x21a, x22a)]"])
-    apply sep_auto
-    done
+interpretation btree_binary_imp_split: imp_split abs_split bin_split
+  apply unfold_locales
+  apply(sep_auto heap: bin_split_imp_abs_split)
   done
 
-
-
-
-(* rebalance middle tree gets a list of trees, an index pointing to
-the position of sub/sep and a last tree *)
-definition rebalance_middle_tree:: "nat \<Rightarrow> (('a::{default,heap,linorder}) btnode ref option \<times> 'a) pfarray \<Rightarrow> nat \<Rightarrow> 'a btnode ref option \<Rightarrow> 'a btnode Heap"
-  where
-    "rebalance_middle_tree \<equiv> \<lambda> k tsi i r_ti. (
-  case r_ti of
-  None \<Rightarrow> do {
-    return (Btnode tsi r_ti)
-  } |
-  Some p_t \<Rightarrow> do {
-      ti \<leftarrow> !p_t;
-      (r_sub,sep) \<leftarrow> pfa_get tsi i;
-      case r_sub of (Some p_sub) \<Rightarrow>  do {
-      sub \<leftarrow> !p_sub;
-      l_sub \<leftarrow> pfa_length (kvs sub);
-      l_ti \<leftarrow> pfa_length (kvs ti);
-      if l_sub \<ge> k \<and> l_ti \<ge> k then do {
-        return (Btnode tsi r_ti)
-      } else do {
-        l_tsi \<leftarrow> pfa_length tsi;
-        if l_tsi = (i+1) then do {
-          mts' \<leftarrow> pfa_append_extend_grow (kvs sub) (last sub,sep) (kvs ti);
-          res_node\<^sub>i \<leftarrow> node\<^sub>i k mts' (last ti);
-          case res_node\<^sub>i of
-            T\<^sub>i u \<Rightarrow> return (Btnode tsi u) |
-            Up\<^sub>i l a r \<Rightarrow> do {
-              tsi' \<leftarrow> pfa_append tsi (l,a);
-              return (Btnode tsi' r)
-            }
-        } else do {
-          (r_rsub,rsep) \<leftarrow> pfa_get tsi (i+1);
-          case r_rsub of Some p_rsub \<Rightarrow> do {
-            rsub \<leftarrow> !p_rsub;
-            mts' \<leftarrow> pfa_append_extend_grow (kvs sub) (last sub,sep) (kvs rsub);
-            res_node\<^sub>i \<leftarrow> node\<^sub>i k mts' (last rsub);
-            case res_node\<^sub>i of
-             T\<^sub>i u \<Rightarrow> do {
-              tsi' \<leftarrow> pfa_set tsi (i+1) (u,rsep);              
-              tsi'' \<leftarrow> pfa_delete tsi' i;
-              return (Btnode tsi'' r_ti)
-            } |
-             Up\<^sub>i l a r \<Rightarrow> do {
-              tsi' \<leftarrow> pfa_set tsi i (l,a);
-              tsi'' \<leftarrow> pfa_set tsi' (i+1) (r,rsep);
-              return (Btnode tsi'' r_ti)
-            }
-          }
-        }
-      }
-  }
-})
-"
-
-definition rebalance_last_tree:: "nat \<Rightarrow> (('a::{default,heap,linorder}) btnode ref option \<times> 'a) pfarray \<Rightarrow> 'a btnode ref option \<Rightarrow> 'a btnode Heap"
-  where
-    "rebalance_last_tree \<equiv> \<lambda>k tsi ti. do {
-   l_tsi \<leftarrow> pfa_length tsi;
-   rebalance_middle_tree k tsi (l_tsi-1) ti
-}"
-
-partial_function (heap) split_max ::"nat \<Rightarrow> ('a::{default,heap,linorder}) btnode ref option \<Rightarrow> ('a btnode ref option \<times> 'a) Heap"
-  where
-    "split_max k r_t = (case r_t of Some p_t \<Rightarrow> do {
-   t \<leftarrow> !p_t;
-   (case t of Btnode tsi r_ti \<Rightarrow>
-     case r_ti of None \<Rightarrow> do {
-      (sub,sep) \<leftarrow> pfa_last tsi;
-      tsi' \<leftarrow> pfa_butlast tsi;
-      p_t := Btnode tsi' sub;
-      return (Some p_t, sep)
-  } |
-    _ \<Rightarrow> do {
-      (sub,sep) \<leftarrow> split_max k r_ti;
-      p_t' \<leftarrow> rebalance_last_tree k tsi sub;
-      p_t := p_t';
-      return (Some p_t, sep)
-  })
-})
-"
-
-partial_function (heap) del ::"nat \<Rightarrow> 'a \<Rightarrow> ('a::{default,heap,linorder}) btnode ref option \<Rightarrow> 'a btnode ref option Heap"
-  where
-    "del k x ti = (case ti of None \<Rightarrow> return None |
-   Some p \<Rightarrow> do {
-   node \<leftarrow> !p;
-   i \<leftarrow> lin_split (kvs node) x;
-   tsl \<leftarrow> pfa_length (kvs node);
-   if i < tsl then do {
-     s \<leftarrow> pfa_get (kvs node) i;
-     let (sub,sep) = s in
-     if x \<noteq> sep then do {
-       sub' \<leftarrow> del k x sub;
-       kvs' \<leftarrow> pfa_set (kvs node) i (sub',sep);
-       node' \<leftarrow> rebalance_middle_tree k kvs' i (last node);
-       ti' \<leftarrow> ref node';
-       return (Some ti')
-      }
-     else if sub = None then do{
-       pfa_delete (kvs node) i;
-       return ti
-     }
-     else do {
-        sm \<leftarrow> split_max k sub;
-        kvs' \<leftarrow> pfa_set (kvs node) i sm;
-        node' \<leftarrow> rebalance_middle_tree k kvs' i (last node);
-        ti' \<leftarrow> ref node';
-        return (Some ti')
-     }
-   } else do {
-       t' \<leftarrow> del k x (last node);
-       node' \<leftarrow> rebalance_last_tree k (kvs node) t';
-       ti' \<leftarrow> ref node';
-       return (Some ti')
-    }
-})
-"
-
-partial_function (heap) reduce_root ::"('a::{default,heap,linorder}) btnode ref option \<Rightarrow> 'a btnode ref option Heap"
-  where
-"reduce_root ti = (case ti of
-  None \<Rightarrow> return None |
-  Some p_t \<Rightarrow> do {
-    node \<leftarrow> !p_t;
-    tsl \<leftarrow> pfa_length (kvs node);
-    case tsl of 0 \<Rightarrow> return (last node) |
-    _ \<Rightarrow> return ti
-})"
-
-partial_function (heap) delete ::"nat \<Rightarrow> 'a \<Rightarrow> ('a::{default,heap,linorder}) btnode ref option \<Rightarrow> 'a btnode ref option Heap"
-  where
-"delete k x ti = do {
-  ti' \<leftarrow> del k x ti;
-  reduce_root ti'
-}"
-
-
-partial_function (heap) isin' :: "('a::{heap,linorder}) btnode ref option \<Rightarrow> 'a \<Rightarrow>  bool Heap"
-  where
-    "isin' p x = 
-  (case p of 
-     None \<Rightarrow> return False |
-     (Some a) \<Rightarrow> do {
-       node \<leftarrow> !a;
-       i \<leftarrow> bin_split (kvs node) x;
-       tsl \<leftarrow> pfa_length (kvs node);
-       if i < tsl then do {
-         s \<leftarrow> pfa_get (kvs node) i;
-         let (sub,sep) = s in
-         if x = sep then
-           return True
-         else
-           isin' sub x
-       } else
-           isin (last node) x
-    }
-)"
-
-
-lemma  "sorted_less (inorder t) \<Longrightarrow> <btree_assn k t ti * true> isin ti x <\<lambda>r. btree_assn k t ti * \<up>(btree_abs_search.isin t x = r)>\<^sub>t"
-proof(induction t x arbitrary: ti rule: btree_abs_search.isin.induct)
-  case (1 x)
-  then show ?case
-    apply(subst isin.simps)
-    apply (cases ti)
-    apply (auto simp add: return_cons_rule)
-    done
-next
-  case (2 ts t x)
-  then obtain ls rs where list_split[simp]: "abs_split ts x = (ls,rs)"
-    by (cases "abs_split ts x")
-  then show ?case
-  proof (cases rs)
-    (* NOTE: induction condition trivial here *)
-    case [simp]: Nil
-    show ?thesis
-      apply(subst isin.simps)
-      apply(sep_auto heap: bin_split_imp_abs_split)
-      apply(auto simp add: split_relation_def dest!: sym[of "[]"] mod_starD list_assn_len)[]
-      apply(rule hoare_triple_preI)
-      apply(auto simp add: split_relation_def dest!: sym[of "[]"] mod_starD list_assn_len)[]
-      using 2(3) apply(sep_auto heap: "2.IH"(1)[of ls "[]"] simp add: sorted_wrt_append)
-      done
-  next
-    case [simp]: (Cons h rrs)
-    obtain sub sep where h_split[simp]: "h = (sub,sep)"
-      by (cases h)
-    show ?thesis
-    proof (cases "sep = x")
-      (* NOTE: no induction required here, only vacuous counter cases generated *)
-      case [simp]: True
-      then show ?thesis
-        apply(simp split: list.splits prod.splits)
-        apply(subst isin.simps)
-        apply(sep_auto heap: bin_split_imp_abs_split)
-        apply(rule hoare_triple_preI)
-        apply(auto simp add: split_relation_alt list_assn_append_Cons_left dest!: mod_starD list_assn_len)[]
-        apply(rule hoare_triple_preI)
-        apply(auto simp add: split_relation_def dest!: sym[of "[]"] mod_starD list_assn_len)[]
-        done
-    next
-      case [simp]: False
-      show ?thesis
-        apply(simp split: list.splits prod.splits)
-        apply safe
-        using False apply simp
-        apply(subst isin.simps)
-        apply(sep_auto heap: bin_split_imp_abs_split)
-          (*eliminate vacuous case*)
-        apply(auto simp add: split_relation_alt list_assn_append_Cons_left dest!:  mod_starD list_assn_len)[]
-          (* simplify towards induction step *)
-        apply(auto simp add: split_relation_alt list_assn_append_Cons_left dest!: mod_starD list_assn_len)[]
-
-(* NOTE show that z = (suba, sepa) *)
-        apply(rule norm_pre_ex_rule)+
-        apply(rule hoare_triple_preI)
-        subgoal for p tsi n ti xsi suba sepa zs1 z zs2 _
-          apply(subgoal_tac "z = (suba, sepa)", simp)
-          using 2(3) apply(sep_auto heap:"2.IH"(2)[of ls rs h rrs sub sep] simp add: sorted_wrt_append)
-          using list_split Cons h_split apply simp_all
-            (* proof that previous assumptions hold later *)
-          apply(rule P_imp_Q_implies_P)
-          apply(rule ent_ex_postI[where ?x="(tsi,n)"])
-          apply(rule ent_ex_postI[where ?x="ti"])
-          apply(rule ent_ex_postI[where ?x="(zs1 @ (suba, sepa) # zs2)"])
-          apply(rule ent_ex_postI[where ?x="zs1"])
-          apply(rule ent_ex_postI[where ?x="z"])
-          apply(rule ent_ex_postI[where ?x="zs2"])
-          apply sep_auto
-            (* prove subgoal_tac assumption *)
-          apply (metis (no_types, lifting) list_assn_aux_ineq_len list_assn_len nth_append_length star_false_left star_false_right)
-          done
-            (* eliminate last vacuous case *)
-        apply(rule hoare_triple_preI)
-        apply(auto simp add: split_relation_def dest!: mod_starD list_assn_len)[]
-        done
-    qed
-  qed
-qed
-
-
-term Array.set
-
-partial_function (heap) ins' :: "nat \<Rightarrow> 'a \<Rightarrow> ('a::{heap,linorder,default}) btnode ref option \<Rightarrow> 'a btupi Heap"
-  where
-    "ins' k x p = (case p of
-  None \<Rightarrow> 
-    return (Up\<^sub>i None x None) |
-  (Some a) \<Rightarrow> do {
-    node \<leftarrow> !a;
-    i \<leftarrow> bin_split (kvs node) x;
-    tsl \<leftarrow> pfa_length (kvs node);
-    if i < tsl then do {
-      s \<leftarrow> pfa_get (kvs node) i;
-      let (sub,sep) = s in
-      if sep = x then
-        return (T\<^sub>i p)
-      else do {
-        r \<leftarrow> ins' k x sub;
-        case r of 
-          (T\<^sub>i lp) \<Rightarrow> do {
-            pfa_set (kvs node) i (lp,sep);
-            return (T\<^sub>i p)
-          } |
-          (Up\<^sub>i lp x' rp) \<Rightarrow> do {
-            kvs' \<leftarrow> pfa_set (kvs node) i (rp,sep);
-            kvs'' \<leftarrow> pfa_insert_grow kvs' i (lp,x');
-            node\<^sub>i k kvs'' (last node)
-          }
-        }
-      }
-    else do {
-      r \<leftarrow> ins' k x (last node);
-      case r of 
-        (T\<^sub>i lp) \<Rightarrow> do {
-          a := (Btnode (kvs node) lp);
-          return (T\<^sub>i p)
-        } |
-        (Up\<^sub>i lp x' rp) \<Rightarrow> do {
-          kvs' \<leftarrow> pfa_append_grow' (kvs node) (lp,x');
-          node\<^sub>i k kvs' rp
-        }
-    }
-  }
-)"
-
-declare  btree_abs_search.ins.simps [simp]
-lemma ins'_rule:
-  "sorted_less (inorder t) \<Longrightarrow> <btree_assn k t ti * true>
-  ins' k x ti
-  <\<lambda>r. btupi_assn k (btree_abs_search.ins k x t) r>\<^sub>t"
-proof (induction k x t arbitrary: ti rule: btree_abs_search.ins.induct)
-  case (1 k x)
-  then show ?case
-    apply(subst ins'.simps)
-    apply (sep_auto simp add: pure_app_eq)
-    done
-next
-  case (2 k x ts t)
-  obtain ls rrs where list_split: "abs_split ts x = (ls,rrs)"
-    by (cases "abs_split ts x")
-  have [simp]: "sorted_less (separators ts)"
-    using "2.prems" sorted_inorder_separators by simp
-  have [simp]: "sorted_less (inorder t)"
-    using "2.prems" sorted_inorder_induct_last by simp
-  show ?case
-  proof (cases rrs)
-    case Nil
-    then show ?thesis
-    proof (cases "btree_abs_search.ins k x t")
-      case (T\<^sub>i a)
-      then show ?thesis
-        apply(subst ins'.simps)
-        apply(sep_auto heap: bin_split_imp_abs_split)
-        subgoal for p tsil tsin tti
-          using Nil list_split
-          by (simp add: Imperative_Loops.list_assn_aux_ineq_len split_relation_alt)
-        subgoal for p tsil tsin tti tsi' xb xaa xc sub sep
-          apply(rule hoare_triple_preI)
-          using Nil list_split
-          by (simp add: Imperative_Loops.list_assn_aux_ineq_len split_relation_alt)
-        subgoal for p tsil tsin tti tsi' xb xaa
-          thm "2.IH"(1)[of ls rrs tti]
-          using Nil list_split T\<^sub>i apply(sep_auto split!: list.splits simp add: split_relation_alt
-              heap add: "2.IH"(1)[of ls rrs tti])
-          subgoal for xi
-            apply(cases xi)
-            apply sep_auto
-            apply sep_auto
-            done
-          done
-        done
-    next
-      case (Up\<^sub>i l a r)
-      then show ?thesis
-        apply(subst ins'.simps)
-        apply(sep_auto heap: bin_split_imp_abs_split)
-        subgoal for p tsil tsin tti
-          using Nil list_split
-          by (simp add: Imperative_Loops.list_assn_aux_ineq_len split_relation_alt)                 
-        subgoal for p tsil tsin tti tsi' xb xaa xc sub sep
-          using Nil list_split 
-          by (simp add: Imperative_Loops.list_assn_aux_ineq_len split_relation_alt)
-        subgoal for p tsil tsin tti tsi' xb xaa
-          thm "2.IH"(1)[of ls rrs tti]
-          using Nil list_split Up\<^sub>i apply(sep_auto split!: list.splits simp add: split_relation_alt
-              heap add: "2.IH"(1)[of ls rrs tti])
-          subgoal for xi
-            apply(cases xi)
-            apply sep_auto
-            apply(sep_auto heap add: node\<^sub>i_rule_app)
-            done
-          done
-        done
-    qed
-  next
-    case (Cons a rs)
-    obtain sub sep where a_split: "a = (sub,sep)"
-      by (cases a)
-    then have [simp]: "sorted_less (inorder sub)"
-      using "2.prems" btree_abs_search.split_axioms list_split Cons sorted_inorder_induct_subtree split_def
-      by fastforce
-    then show ?thesis
-    proof(cases "x = sep")
-      case True
-      show ?thesis
-        apply(subst ins'.simps)
-        apply(sep_auto heap: bin_split_imp_abs_split)
-        subgoal for p tsil tsin tti tsi j subi
-          using Cons list_split a_split True
-          by sep_auto
-        subgoal for p tsil tsin tti tsi j _ _ subi sepi
-          apply(rule hoare_triple_preI)
-          using Cons list_split a_split True
-          apply(subgoal_tac "sepi = sep")
-          apply (sep_auto simp add: split_relation_alt)
-          apply(sep_auto simp add: list_assn_prod_map dest!: mod_starD id_assn_list)
-          by (metis length_map snd_conv snd_map_help(2) split_relation_access)
-        subgoal for p tsil tsin tti tsi j
-          apply(rule hoare_triple_preI)
-          using Cons list_split
-          by (sep_auto simp add: split_relation_alt dest!: mod_starD list_assn_len)
-        done
-    next
-      case False
-      then show ?thesis
-      proof (cases "btree_abs_search.ins k x sub")
-        case (T\<^sub>i a')
-        then show ?thesis
-          apply(auto simp add: Cons list_split a_split False)
-          using False apply simp
-          apply(subst ins'.simps)
-          apply vcg
-          apply auto
-          apply(rule norm_pre_ex_rule)+
-            (* at this point, we want to introduce the split, and after that tease the
-  hoare triple assumptions out of the bracket, s.t. we don't split twice *)
-          apply vcg
-          apply sep_auto
-          using list_split Cons
-          apply(simp add: split_relation_alt list_assn_append_Cons_left)
-          apply (rule impI)
-          apply(rule norm_pre_ex_rule)+
-          apply(rule hoare_triple_preI)
-          apply sep_auto
-            (* discard wrong branch *)
-          subgoal for p tsil tsin ti zs1 subi sepi zs2 _ _ suba
-            apply(subgoal_tac "sepi  = x")
-            using list_split Cons a_split
-            apply(auto  dest!:  mod_starD )[]
-            apply(auto dest!:  mod_starD list_assn_len)[]
-            done
-              (* actual induction branch *)
-          subgoal for p tsil tsin ti zs1 subi sepi zs2 _ _ n z suba sepa
-            apply (cases a, simp)
-            apply(subgoal_tac "subi = suba", simp)
-            using list_split a_split T\<^sub>i False
-            apply (vcg heap: 2)
-            apply(auto split!: btupi.splits)
-              (* careful progression for manual value insertion *)
-            apply vcg
-            apply simp
-            apply vcg
-            apply simp
-            subgoal for a'i q r
-              apply(rule impI)
-              apply(simp add: list_assn_append_Cons_left)
-              apply(rule ent_ex_postI[where ?x="(tsil,tsin)"])
-              apply(rule ent_ex_postI[where ?x="ti"])
-              apply(rule ent_ex_postI[where ?x="(zs1 @ (a'i, sepi) # zs2)"])
-              apply(rule ent_ex_postI[where ?x="zs1"])
-              apply(rule ent_ex_postI[where ?x="(a'i,sep)"])
-              apply(rule ent_ex_postI[where ?x="zs2"])
-              apply sep_auto
-              apply (simp add: pure_app_eq)
-              apply(sep_auto dest!:  mod_starD list_assn_len)[]
-              done
-            apply (metis Imperative_Loops.list_assn_aux_ineq_len Pair_inject list_assn_len nth_append_length star_false_left star_false_right)
-            done
-          subgoal for p tsil tsin ti zs1 subi sepi zs2 _ _ suba
-            apply(auto dest!:  mod_starD list_assn_len)[]
-            done
-          done
-      next
-        case (Up\<^sub>i l w r)
-        then show ?thesis
-          apply(auto simp add: Cons list_split a_split False)
-          using False apply simp
-          apply(subst ins'.simps)
-          apply vcg
-          apply auto
-          apply(rule norm_pre_ex_rule)+
-            (* at this point, we want to introduce the split, and after that tease the
-  hoare triple assumptions out of the bracket, s.t. we don't split twice *)
-          apply vcg
-          apply sep_auto
-          using list_split Cons
-          apply(simp add: split_relation_alt list_assn_append_Cons_left)
-          apply (rule impI)
-          apply(rule norm_pre_ex_rule)+
-          apply(rule hoare_triple_preI)
-          apply sep_auto
-            (* discard wrong branch *)
-          subgoal for p tsil tsin ti zs1 subi sepi zs2 _ _ suba
-            apply(subgoal_tac "sepi  = x")
-            using list_split Cons a_split
-            apply(auto  dest!:  mod_starD )[]
-            apply(auto dest!:  mod_starD list_assn_len)[]
-            done
-              (* actual induction branch *)
-          subgoal for p tsil tsin ti zs1 subi sepi zs2 _ _ n z suba sepa
-            apply(subgoal_tac "subi = suba", simp)
-            thm 2(2)[of ls rrs a rs sub sep]
-            using list_split a_split Cons Up\<^sub>i False
-            apply (sep_auto heap: 2(2))
-            apply(auto split!: btupi.splits)
-              (* careful progression for manual value insertion *)
-            apply vcg
-            apply simp
-            subgoal for x21 x22 x23 u
-              apply (cases u,simp)
-              thm pfa_insert_grow_rule[where ?l="((zs1 @ (suba, sepi) # zs2)[length ls := (x23, sepa)])"]
-              apply (sep_auto dest!: mod_starD list_assn_len heap: pfa_insert_grow_rule)
-              apply (simp add: is_pfa_def)[]
-              apply (metis le_less_linear length_append length_take less_not_refl min.absorb2 trans_less_add1)
-              apply(auto split: prod.splits  dest!: mod_starD list_assn_len)[]
-
-              apply (vcg heap: node\<^sub>i_rule_ins2)
-              apply simp
-              apply simp
-              apply simp
-              apply sep_auto
-              done
-            apply(auto dest!:  mod_starD list_assn_len)[]
-            done
-          subgoal for p tsil tsin ti zs1 subi sepi zs2 _ _ suba
-            apply(auto dest!:  mod_starD list_assn_len)[]
-            done
-          done
-      qed
-    qed
-  qed
-qed
-
-declare btree_abs_search.ins.simps[simp del]
-
-(*fun tree\<^sub>i::"'a up\<^sub>i \<Rightarrow> 'a btree" where
-  "tree\<^sub>i (T\<^sub>i sub) = sub" |
-  "tree\<^sub>i (Up\<^sub>i l a r) = (Node [(l,a)] r)" 
-
-fun insert::"nat \<Rightarrow> 'a \<Rightarrow> 'a btree \<Rightarrow> 'a btree" where
-  "insert k x t = tree\<^sub>i (ins k x t)"
-*)
-
-definition insert' :: "nat \<Rightarrow> ('a::{heap,default,linorder}) \<Rightarrow> 'a btnode ref option \<Rightarrow> 'a btnode ref option Heap" where
-  "insert' \<equiv> \<lambda>k x ti. do {
-  ti' \<leftarrow> ins' k x ti;
-  case ti' of
-     T\<^sub>i sub \<Rightarrow> return sub |
-     Up\<^sub>i l a r \<Rightarrow> do {
-        kvs \<leftarrow> pfa_init (2*k) (l,a) 1;
-        t' \<leftarrow> ref (Btnode kvs r);
-        return (Some t')
-      }
-}"
-
-lemma insert'_rule:
-  assumes "k > 0" "sorted_less (inorder t)"
-  shows "<btree_assn k t ti * true>
-  insert' k x ti
-  <\<lambda>r. btree_assn k (btree_abs_search.insert k x t) r>\<^sub>t"
-  unfolding insert'_def
-  apply(cases "btree_abs_search.ins k x t")
-  apply(sep_auto split!: btupi.splits heap: ins'_rule[OF assms(2)])
-  using assms
-  apply(vcg heap: ins'_rule[OF assms(2)])
-  apply(simp split!: btupi.splits)
-  apply(vcg)
-  apply simp
-  apply simp
-  apply vcg
-  apply auto[]
-  subgoal for x21 x22 x23 x21a x22a x23a a b xa
-    apply(rule ent_ex_postI[where ?x="(a,b)"])
-    apply(rule ent_ex_postI[where ?x="x23a"])
-    apply(rule ent_ex_postI[where ?x="[(x21a, x22a)]"])
-    apply sep_auto
-    done
+definition [code del]: "binary_imp_ins = btree_binary_imp_split.ins"
+lemma [code]: "binary_imp_ins k x p = (
+      case p of None \<Rightarrow> return (btree_binary_imp_split.Up\<^sub>i None x None)
+     | Some a \<Rightarrow> do {
+           node \<leftarrow> !a;
+           i \<leftarrow> bin_split (kvs node) x;
+           tsl \<leftarrow> pfa_length (kvs node);
+           if i < tsl
+           then do {
+                  s \<leftarrow> pfa_get (kvs node) i;
+                  let (sub, sep) = s;
+                  if sep = x then return (btree_binary_imp_split.T\<^sub>i p)
+                  else do {
+                         r \<leftarrow> binary_imp_ins k x sub;
+                         case r of btree_binary_imp_split.T\<^sub>i lp \<Rightarrow> do {
+                                       _ \<leftarrow> pfa_set (kvs node) i (lp, sep);
+                                       return (btree_binary_imp_split.T\<^sub>i p)
+                                     }
+                         | btree_binary_imp_split.Up\<^sub>i lp x' rp \<Rightarrow> do {
+                               kvs' \<leftarrow> pfa_set (kvs node) i (rp, sep);
+                               kvs'' \<leftarrow> pfa_insert_grow kvs' i (lp, x');
+                               btree_binary_imp_split.node\<^sub>i k kvs'' (BTree_Imp.last node)
+                             }
+                       }
+                }
+           else do {
+                  r \<leftarrow> binary_imp_ins k x (BTree_Imp.last node);
+                  case r of btree_binary_imp_split.T\<^sub>i lp \<Rightarrow> do {
+                                _ \<leftarrow> a := Btnode (kvs node) lp;
+                                return (btree_binary_imp_split.T\<^sub>i p)
+                              }
+                  | btree_binary_imp_split.Up\<^sub>i lp x' rp \<Rightarrow> do {
+                        kvs' \<leftarrow> pfa_append_grow' (kvs node) (lp, x');
+                        btree_binary_imp_split.node\<^sub>i k kvs' rp
+                      }
+                }
+         })"
+  apply (subst binary_imp_ins_def)+
+  apply (simp add: btree_binary_imp_split.ins.simps)
   done
+  
+definition [code del]: "binary_imp_insert = btree_binary_imp_split.insert"
+lemma [code]: "binary_imp_insert = (\<lambda>k x ti. do {
+         ti' \<leftarrow> binary_imp_ins k x ti;
+         case ti' of btree_binary_imp_split.T\<^sub>i sub \<Rightarrow> return sub
+         | btree_binary_imp_split.Up\<^sub>i l a r \<Rightarrow> do {
+               kvs \<leftarrow> pfa_init (2 * k) (l, a) 1;
+               t' \<leftarrow> ref (Btnode kvs r);
+               return (Some t')
+             }
+       })"
+  by (simp add: binary_imp_ins_def binary_imp_insert_def  btree_binary_imp_split.insert_def)
+
+
+export_code binary_imp_insert checking SML Scala
+export_code binary_imp_insert in SML module_name BTreeInsert
 
 
 end
